Bdd/Evaluate.lean
@@ -16,7 +16,7 @@ lemma evaluate_evaluate : evaluate O = OBdd.evaluate O := by
   ext I
   unfold evaluate
   split
-  next b hb => simp [OBdd.evaluate_terminal' hb]
+  next b hb => simp [OBdd.evaluate_terminal hb]
   next j hj =>
     have := evaluate_evaluate (O := O.low hj)
     have := evaluate_evaluate (O := O.high hj)
@@ -25,7 +25,7 @@ termination_by O
 
 lemma evaluate_terminal {O : OBdd n m} : O.1.root = .terminal b → evaluate O = Function.const _ b := by
   rw [evaluate_evaluate]
-  exact OBdd.evaluate_terminal'
+  exact OBdd.evaluate_terminal
 
 lemma evaluate_node {O : OBdd n m} (h : O.1.root = .node j) :
     evaluate O = fun I ↦ if I[O.1.heap[j].var] then evaluate (O.high h) I else evaluate (O.low h) I := by
